Primitive_Matchers/IpAddresses.thy
@@ -19,21 +19,21 @@ done
 
 subsection{*IPv4 Addresses in CIDR Notation*}
   (*We need a separate ipv4addr syntax thy*)
-  fun ipv4cidr_to_intervall :: "(ipv4addr \<times> nat) \<Rightarrow> (ipv4addr \<times> ipv4addr)" where
-    "ipv4cidr_to_intervall (pre, len) = (
+  fun ipv4cidr_to_interval :: "(ipv4addr \<times> nat) \<Rightarrow> (ipv4addr \<times> ipv4addr)" where
+    "ipv4cidr_to_interval (pre, len) = (
       let netmask = (mask len) << (32 - len);
           network_prefix = (pre AND netmask)
       in (network_prefix, network_prefix OR (NOT netmask))
      )"
-  lemma ipv4cidr_to_intervall: "ipv4cidr_to_intervall (base, len) = (s,e) \<Longrightarrow> ipv4range_set_from_bitmask base len = {s .. e}"
+  lemma ipv4cidr_to_interval: "ipv4cidr_to_interval (base, len) = (s,e) \<Longrightarrow> ipv4range_set_from_bitmask base len = {s .. e}"
     apply(simp add: Let_def)
     apply(subst ipv4range_set_from_bitmask_alt)
     apply(subst(asm) NOT_mask_len32)
     by (metis NOT_mask_len32 ipv4range_set_from_bitmask_alt ipv4range_set_from_bitmask_alt1 ipv4range_set_from_netmask_def)
-  declare ipv4cidr_to_intervall.simps[simp del]
+  declare ipv4cidr_to_interval.simps[simp del]
 
-  fun simple_ips_conjunct :: "(ipv4addr \<times> nat) \<Rightarrow> (ipv4addr \<times> nat) \<Rightarrow> (ipv4addr \<times> nat) option" where 
-    "simple_ips_conjunct (base1, m1) (base2, m2) = (if ipv4range_set_from_bitmask base1 m1 \<inter> ipv4range_set_from_bitmask base2 m2 = {}
+  fun ipv4cidr_conjunct :: "(ipv4addr \<times> nat) \<Rightarrow> (ipv4addr \<times> nat) \<Rightarrow> (ipv4addr \<times> nat) option" where 
+    "ipv4cidr_conjunct (base1, m1) (base2, m2) = (if ipv4range_set_from_bitmask base1 m1 \<inter> ipv4range_set_from_bitmask base2 m2 = {}
        then
         None
        else if 
@@ -44,25 +44,26 @@ subsection{*IPv4 Addresses in CIDR Notation*}
         Some (base2, m2)
       )"
   
-  lemma simple_ips_conjunct_correct: "(case simple_ips_conjunct (b1, m1) (b2, m2) of Some (bx, mx) \<Rightarrow> ipv4range_set_from_bitmask bx mx | None \<Rightarrow> {}) = 
+  lemma ipv4cidr_conjunct_correct: "(case ipv4cidr_conjunct (b1, m1) (b2, m2) of Some (bx, mx) \<Rightarrow> ipv4range_set_from_bitmask bx mx | None \<Rightarrow> {}) = 
       (ipv4range_set_from_bitmask b1 m1) \<inter> (ipv4range_set_from_bitmask b2 m2)"
     apply(simp split: split_if_asm)
     using ipv4range_bitmask_intersect by fast
-  declare simple_ips_conjunct.simps[simp del]
+  declare ipv4cidr_conjunct.simps[simp del]
 
-  definition ipv4_cidr_tuple_to_intervall :: "(ipv4addr \<times> nat) \<Rightarrow> 32 wordinterval" where
-    "ipv4_cidr_tuple_to_intervall base_len = (case ipv4cidr_to_intervall base_len of (s,e) \<Rightarrow> ipv4range_range s e)"
+  definition ipv4_cidr_tuple_to_interval :: "(ipv4addr \<times> nat) \<Rightarrow> 32 wordinterval" where
+    "ipv4_cidr_tuple_to_interval iprng = ipv4range_range (ipv4cidr_to_interval iprng)"
 
-  lemma ipv4range_to_set_ipv4_cidr_tuple_to_intervall: "ipv4range_to_set (ipv4_cidr_tuple_to_intervall (b, m)) = ipv4range_set_from_bitmask b m"
-    unfolding ipv4_cidr_tuple_to_intervall_def
-    by(simp add: ipv4cidr_to_intervall ipv4range_range_set_eq split: split_split)
+  lemma ipv4range_to_set_ipv4_cidr_tuple_to_interval: "ipv4range_to_set (ipv4_cidr_tuple_to_interval (b, m)) = ipv4range_set_from_bitmask b m"
+    unfolding ipv4_cidr_tuple_to_interval_def
+    apply(cases "ipv4cidr_to_interval (b, m)")
+    using ipv4cidr_to_interval ipv4range_range_set_eq by presburger
 
   lemma [code_unfold]: 
-  "simple_ips_conjunct ips1 ips2 = (if ipv4range_empty (ipv4range_intersection (ipv4_cidr_tuple_to_intervall ips1) (ipv4_cidr_tuple_to_intervall ips2))
+  "ipv4cidr_conjunct ips1 ips2 = (if ipv4range_empty (ipv4range_intersection (ipv4_cidr_tuple_to_interval ips1) (ipv4_cidr_tuple_to_interval ips2))
        then
         None
        else if 
-        ipv4range_subset (ipv4_cidr_tuple_to_intervall ips1) (ipv4_cidr_tuple_to_intervall ips2)
+        ipv4range_subset (ipv4_cidr_tuple_to_interval ips1) (ipv4_cidr_tuple_to_interval ips2)
        then 
         Some ips1
        else
@@ -71,11 +72,14 @@ subsection{*IPv4 Addresses in CIDR Notation*}
   apply(simp)
   apply(cases ips1, cases ips2, rename_tac b1 m1 b2 m2, simp)
   apply(safe)
-     apply(simp_all add: ipv4range_to_set_ipv4_cidr_tuple_to_intervall simple_ips_conjunct.simps split:split_if_asm)
+     apply(simp_all add: ipv4range_to_set_ipv4_cidr_tuple_to_interval ipv4cidr_conjunct.simps split:split_if_asm)
     apply fast+
   done
-  value "simple_ips_conjunct (0,0) (8,1)" (*with the code_unfold lema before, this works!*)
+  value "ipv4cidr_conjunct (0,0) (8,1)" (*with the code_unfold lema before, this works!*)
 
+
+  definition ipv4cidr_union_set :: "(ipv4addr \<times> nat) set \<Rightarrow> ipv4addr set" where
+    "ipv4cidr_union_set ips \<equiv> \<Union>(base, len) \<in> ips. ipv4range_set_from_bitmask base len"
 
 
 
@@ -109,33 +113,33 @@ subsection{*IPv4 Addresses in IPTables Notation (how we parse it)*}
   
 
   text{*IPv4 address ranges to @{text "(start, end)"} notation*}
-  fun ipt_ipv4range_to_intervall :: "ipt_ipv4range \<Rightarrow> (ipv4addr \<times> ipv4addr)" where
-    "ipt_ipv4range_to_intervall (Ip4Addr addr) = (ipv4addr_of_dotdecimal addr, ipv4addr_of_dotdecimal addr)" |
-    "ipt_ipv4range_to_intervall (Ip4AddrNetmask pre len) = ipv4cidr_to_intervall ((ipv4addr_of_dotdecimal pre), len)" 
+  fun ipt_ipv4range_to_interval :: "ipt_ipv4range \<Rightarrow> (ipv4addr \<times> ipv4addr)" where
+    "ipt_ipv4range_to_interval (Ip4Addr addr) = (ipv4addr_of_dotdecimal addr, ipv4addr_of_dotdecimal addr)" |
+    "ipt_ipv4range_to_interval (Ip4AddrNetmask pre len) = ipv4cidr_to_interval ((ipv4addr_of_dotdecimal pre), len)" 
   
-  lemma ipt_ipv4range_to_intervall: "ipt_ipv4range_to_intervall ip = (s,e) \<Longrightarrow> {s .. e} = ipv4s_to_set ip"
-    by(cases ip) (auto simp add: ipv4cidr_to_intervall)
+  lemma ipt_ipv4range_to_interval: "ipt_ipv4range_to_interval ip = (s,e) \<Longrightarrow> {s .. e} = ipv4s_to_set ip"
+    by(cases ip) (auto simp add: ipv4cidr_to_interval)
 
   text{*A list of IPv4 address ranges to a @{typ "32 wordinterval"}.
         The nice thing is: the usual set operations are defined on this type.
         We can use the existing function @{const l2br_intersect} if we want the intersection of the supplied list*}
-  lemma "wordinterval_to_set (l2br_intersect (map ipt_ipv4range_to_intervall ips)) = (\<Inter> ip \<in> set ips. ipv4s_to_set ip)"
+  lemma "wordinterval_to_set (l2br_intersect (map ipt_ipv4range_to_interval ips)) = (\<Inter> ip \<in> set ips. ipv4s_to_set ip)"
     apply(simp add: l2br_intersect)
-    using ipt_ipv4range_to_intervall by blast
+    using ipt_ipv4range_to_interval by blast
   
   text{*We can use @{const l2br} if we want the union of the supplied list*}
-  lemma "wordinterval_to_set (l2br (map ipt_ipv4range_to_intervall ips)) = (\<Union> ip \<in> set ips. ipv4s_to_set ip)"
+  lemma "wordinterval_to_set (l2br (map ipt_ipv4range_to_interval ips)) = (\<Union> ip \<in> set ips. ipv4s_to_set ip)"
     apply(simp add: l2br)
-    using ipt_ipv4range_to_intervall by blast
+    using ipt_ipv4range_to_interval by blast
 
   text{*A list of (negated) IPv4 address to a @{typ "32 wordinterval"}.*}
   definition ipt_ipv4range_negation_type_to_br_intersect :: "ipt_ipv4range negation_type list \<Rightarrow> 32 wordinterval" where
-    "ipt_ipv4range_negation_type_to_br_intersect l = l2br_negation_type_intersect (NegPos_map ipt_ipv4range_to_intervall l)" 
+    "ipt_ipv4range_negation_type_to_br_intersect l = l2br_negation_type_intersect (NegPos_map ipt_ipv4range_to_interval l)" 
 
   lemma ipt_ipv4range_negation_type_to_br_intersect: "wordinterval_to_set (ipt_ipv4range_negation_type_to_br_intersect l) =
       (\<Inter> ip \<in> set (getPos l). ipv4s_to_set ip) - (\<Union> ip \<in> set (getNeg l). ipv4s_to_set ip)"
     apply(simp add: ipt_ipv4range_negation_type_to_br_intersect_def l2br_negation_type_intersect NegPos_map_simps)
-    using ipt_ipv4range_to_intervall by blast
+    using ipt_ipv4range_to_interval by blast
 
   text{*The @{typ "32 wordinterval"} can be translated back into a list of IP ranges.
         If a list of intervals is enough, we can use @{const br2l}.
