Simple_Firewall/SimpleFw_Compliance.thy
@@ -67,8 +67,8 @@ text{*@{typ "simple_match"} @{text \<and>} @{typ "simple_match"}*}
   fun simple_match_and :: "simple_match \<Rightarrow> simple_match \<Rightarrow> simple_match option" where
     "simple_match_and \<lparr>iiface=iif1, oiface=oif1, src=sip1, dst=dip1, proto=p1, sports=sps1, dports=dps1 \<rparr> 
                       \<lparr>iiface=iif2, oiface=oif2, src=sip2, dst=dip2, proto=p2, sports=sps2, dports=dps2 \<rparr> = 
-      (case simple_ips_conjunct sip1 sip2 of None \<Rightarrow> None | Some sip \<Rightarrow> 
-      (case simple_ips_conjunct dip1 dip2 of None \<Rightarrow> None | Some dip \<Rightarrow> 
+      (case ipv4cidr_conjunct sip1 sip2 of None \<Rightarrow> None | Some sip \<Rightarrow> 
+      (case ipv4cidr_conjunct dip1 dip2 of None \<Rightarrow> None | Some dip \<Rightarrow> 
       (case iface_conjunct iif1 iif2 of None \<Rightarrow> None | Some iif \<Rightarrow>
       (case iface_conjunct oif1 oif2 of None \<Rightarrow> None | Some oif \<Rightarrow>
       (case simple_proto_conjunct p1 p2 of None \<Rightarrow> None | Some p \<Rightarrow>
@@ -83,14 +83,14 @@ text{*@{typ "simple_match"} @{text \<and>} @{typ "simple_match"}*}
     obtain iif2 oif2 sip2 dip2 p2 sps2 dps2 where m2:
       "m2 = \<lparr>iiface=iif2, oiface=oif2, src=sip2, dst=dip2, proto=p2, sports=sps2, dports=dps2 \<rparr>" by(cases m2, blast)
 
-    have sip_None: "simple_ips_conjunct sip1 sip2 = None \<Longrightarrow> \<not> simple_match_ip sip1 (p_src p) \<or> \<not> simple_match_ip sip2 (p_src p)"
+    have sip_None: "ipv4cidr_conjunct sip1 sip2 = None \<Longrightarrow> \<not> simple_match_ip sip1 (p_src p) \<or> \<not> simple_match_ip sip2 (p_src p)"
       using simple_match_ip_conjunct[of sip1 "p_src p" sip2] by simp
-    have dip_None: "simple_ips_conjunct dip1 dip2 = None \<Longrightarrow> \<not> simple_match_ip dip1 (p_dst p) \<or> \<not> simple_match_ip dip2 (p_dst p)"
+    have dip_None: "ipv4cidr_conjunct dip1 dip2 = None \<Longrightarrow> \<not> simple_match_ip dip1 (p_dst p) \<or> \<not> simple_match_ip dip2 (p_dst p)"
       using simple_match_ip_conjunct[of dip1 "p_dst p" dip2] by simp
-    have sip_Some: "\<And>ip. simple_ips_conjunct sip1 sip2 = Some ip \<Longrightarrow>
+    have sip_Some: "\<And>ip. ipv4cidr_conjunct sip1 sip2 = Some ip \<Longrightarrow>
       simple_match_ip ip (p_src p) \<longleftrightarrow> simple_match_ip sip1 (p_src p) \<and> simple_match_ip sip2 (p_src p)"
       using simple_match_ip_conjunct[of sip1 "p_src p" sip2] by simp
-    have dip_Some: "\<And>ip. simple_ips_conjunct dip1 dip2 = Some ip \<Longrightarrow>
+    have dip_Some: "\<And>ip. ipv4cidr_conjunct dip1 dip2 = Some ip \<Longrightarrow>
       simple_match_ip ip (p_dst p) \<longleftrightarrow> simple_match_ip dip1 (p_dst p) \<and> simple_match_ip dip2 (p_dst p)"
       using simple_match_ip_conjunct[of dip1 "p_dst p" dip2] by simp
 
