Simple_Firewall/SimpleFw_Semantics.thy
@@ -126,19 +126,19 @@ subsection{*Simple Ports*}
 
 subsection{*Simple IPs*}
   lemma simple_match_ip_conjunct: "simple_match_ip ip1 p_ip \<and> simple_match_ip ip2 p_ip \<longleftrightarrow> 
-         (case simple_ips_conjunct ip1 ip2 of None \<Rightarrow> False | Some ipx \<Rightarrow> simple_match_ip ipx p_ip)"
+         (case ipv4cidr_conjunct ip1 ip2 of None \<Rightarrow> False | Some ipx \<Rightarrow> simple_match_ip ipx p_ip)"
   proof -
   {
     fix b1 m1 b2 m2
     have "simple_match_ip (b1, m1) p_ip \<and> simple_match_ip (b2, m2) p_ip \<longleftrightarrow> 
           p_ip \<in> ipv4range_set_from_bitmask b1 m1 \<inter> ipv4range_set_from_bitmask b2 m2"
     by simp
-    also have "\<dots> \<longleftrightarrow> p_ip \<in> (case simple_ips_conjunct (b1, m1) (b2, m2) of None \<Rightarrow> {} | Some (bx, mx) \<Rightarrow> ipv4range_set_from_bitmask bx mx)"
-      using simple_ips_conjunct_correct by blast
-    also have "\<dots> \<longleftrightarrow> (case simple_ips_conjunct (b1, m1) (b2, m2) of None \<Rightarrow> False | Some ipx \<Rightarrow> simple_match_ip ipx p_ip)"
+    also have "\<dots> \<longleftrightarrow> p_ip \<in> (case ipv4cidr_conjunct (b1, m1) (b2, m2) of None \<Rightarrow> {} | Some (bx, mx) \<Rightarrow> ipv4range_set_from_bitmask bx mx)"
+      using ipv4cidr_conjunct_correct by blast
+    also have "\<dots> \<longleftrightarrow> (case ipv4cidr_conjunct (b1, m1) (b2, m2) of None \<Rightarrow> False | Some ipx \<Rightarrow> simple_match_ip ipx p_ip)"
       by(simp split: option.split)
     finally have "simple_match_ip (b1, m1) p_ip \<and> simple_match_ip (b2, m2) p_ip \<longleftrightarrow> 
-         (case simple_ips_conjunct (b1, m1) (b2, m2) of None \<Rightarrow> False | Some ipx \<Rightarrow> simple_match_ip ipx p_ip)" .
+         (case ipv4cidr_conjunct (b1, m1) (b2, m2) of None \<Rightarrow> False | Some ipx \<Rightarrow> simple_match_ip ipx p_ip)" .
    } thus ?thesis by(cases ip1, cases ip2, simp)
   qed
 
